

#	Before mtext processing	After change mtext to mspace (changed equations only)
222	$M(X) = A_r(X) [M(^{12}C) / 12] = A_r(X) M_u$	$M(X) = A_r(X) [M(^{12}C) / 12] = A_r(X) M_u$
848	$5s^2S_{1/2}-4d^2D_{5/2}$	$5s^2S_{1/2}-4d^2D_{5/2}$
851	$5d^{10}6s^2S_{1/2}(F=0)-5d^96s^2D_{5/2}(F=2)$	$5d^{10}6s^2S_{1/2}(F=0)-5d^96s^2D_{5/2}(F=2)$
854	$6s^2S_{1/2}(F=0)-5d^2D_{3/2}(F=2)$	$6s^2S_{1/2}(F=0)-5d^2D_{3/2}(F=2)$
857	$5s^2_1S_0-5s5p^3P_0$	$5s^2_1S_0-5s5p^3P_0$
872	$5s^2_1S_0-5s5p^3P_0$	$5s^2_1S_0-5s5p^3P_0$
875	$5s^2_1S_0-5s5p^3P_0$	$5s^2_1S_0-5s5p^3P_0$
878	$4s^2S_{1/2}-3d^2D_{5/2}$	$4s^2S_{1/2}-3d^2D_{5/2}$
881	$(F=0)^{-2}F_{7/2}(F=3, m_F=0)$	$(F=0)^{-2}F_{7/2}(F=3, m_F=0)$
884	$6s^2_1S_0(F=1/2)-6s6p^3P_0(F=1/2)$	$6s^2_1S_0(F=1/2)-6s6p^3P_0(F=1/2)$
973	$6s^2_1S_0-6s6p^3P_0$	$6s^2_1S_0-6s6p^3P_0$
976	$4s^2S_{1/2}-3d^2D_{5/2}$	$4s^2S_{1/2}-3d^2D_{5/2}$
984	$6s^2S_{1/2}-4f^{13}6s^2F_{7/2}$	$6s^2S_{1/2}-4f^{13}6s^2F_{7/2}$
987	$6s^2_1S_0-6s6p^3P_0$	$6s^2_1S_0-6s6p^3P_0$
990	$3s^2_1S_0-3s3p^3P_0$	$3s^2_1S_0-3s3p^3P_0$
993	$5d^{10}6s^2S_{1/2}-5d^96s^2D_{5/2}$	$5d^{10}6s^2S_{1/2}-5d^96s^2D_{5/2}$
996	$6s^2S_{1/2}(F=0, m_F=0)-5d^2D_{3/2}(F=2, m_F=0)$	$6s^2S_{1/2}(F=0, m_F=0)-5d^2D_{3/2}(F=2, m_F=0)$
999	$5s^2S_{1/2}-4d^2D_{5/2}$	$5s^2S_{1/2}-4d^2D_{5/2}$
1002	$5s^2_1S_0-5s5p^3P_0$	$5s^2_1S_0-5s5p^3P_0$
1018	$6s^2_1S_0-6s6p^3P_0$	$6s^2_1S_0-6s6p^3P_0$
1021	$6s^2S_{1/2}-4f^{13}6s^2F_{7/2}$	$6s^2S_{1/2}-4f^{13}6s^2F_{7/2}$
1024	$6s^2S_{1/2}(F=0, m_F=0)-5d^2D_{3/2}(F=2, m_F=0)$	$6s^2S_{1/2}(F=0, m_F=0)-5d^2D_{3/2}(F=2, m_F=0)$
1027	$5s^2S_{1/2}-4d^2D_{5/2}$	$5s^2S_{1/2}-4d^2D_{5/2}$
1030	$4s^2S_{1/2}-3d^2D_{5/2}$	$4s^2S_{1/2}-3d^2D_{5/2}$
1038	$5s^2_1S_0-5s5p^3P_0$	$5s^2_1S_0-5s5p^3P_0$
1041	$6s^2_1S_0-6s6p^3P_0$	$6s^2_1S_0-6s6p^3P_0$